split theories into Abstract, Concrete, Refinement

examples/spinlock/spinlockRefinementScript.sml
@@ -3,371 +3,21 @@ open HolKernel Parse boolLib bossLib;
 open rich_listTheory listTheory arithmeticTheory finite_mapTheory ;
 open bir_lifter_interfaceLib ;
 open bir_promisingTheory ;
-open tracesTheory
-(* tracestepTheory spinlockTheory ; *)
+open tracesTheory spinlockAbstractTheory spinlockConcreteTheory;
 
 val _ = new_theory "spinlockRefinement";
-
-(*****************************************************************************)
-(* The full spinlock program *************************************************)
-(*****************************************************************************)
-
-val _ = set_trace "bir_inst_lifting.DEBUG_LEVEL" 2;
-
-val (bir_spinlockfull_progbin_def, bir_spinlockfull_prog_def, bir_is_lifted_prog_spinlockfull) = lift_da_and_store_mc_riscv
-          "spinlockfull"
-          "spinlockfull.da"
-          ((Arbnum.fromInt 0), (Arbnum.fromInt 0x1000000));
-
-(*****************************************************************************)
-(* Helper definitions ********************************************************)
-(*****************************************************************************)
-(* TODO place these elsewhere *)
-
-(* projection of the state of a core *)
-
-Definition core_def:
-  core cid S = THE $ FLOOKUP (FST S) cid
-End
-
-Definition core_state_def:
-  core_state cid S = get_core_state $ core cid S
-End
-
-Definition core_prog_def:
-  core_prog cid S = get_core_prog $ core cid S
-End
-
-Definition bst_pc_tuple_def:
-  bst_pc_tuple x = (x.bpc_label,x.bpc_index)
-End
-
-Definition core_pc_def:
-  core_pc cid S = (core_state cid S).bst_pc
-End
-
-(* read a variable from a given memory *)
-
-Definition bir_read_mem_var_def:
-  bir_read_mem_var mem var env =
-    bir_eval_exp
-      (BExp_Load (BExp_Den $ BVar mem $ BType_Mem Bit64 Bit8)
-        (BExp_Den $ BVar var $ BType_Imm Bit64)
-        BEnd_LittleEndian Bit32) env
-End
-
-(* read a variable from an environment  *)
-
-Definition bir_read_var_def:
-  bir_read_var var env =
-    bir_eval_exp (BExp_Den (BVar var (BType_Imm Bit64))) env
-End
-
-(* read a variable from a core state *)
-
-Definition bir_read_core_reg_def:
-  bir_read_core_reg var cid S =
-    bir_read_var var (core_state cid S).bst_environ
-End
-
-(* read a zero variable from a core state *)
-
-Definition bir_read_core_reg_zero_def:
-  bir_read_core_reg_zero var cid S <=>
-    bir_read_core_reg var cid S = SOME $ BVal_Imm $ Imm64 0w
-End
-
-(* compare address range *)
-
-Definition bir_laImm64_lt_def:
-  bir_laImm64_lt a w =
-    case a of
-    | BL_Address (Imm64 v) => v < w
-    | _ => F
-End
-
-Definition bir_laImm64_lt2_def:
-  bir_laImm64_lt2 w a =
-    case a of
-    | BL_Address (Imm64 v) => w < v
-    | _ => F
-End
-
-(*****************************************************************************)
-(* Extracting reachable states of a program **********************************)
-(*****************************************************************************)
-(* TODO some theorems need further adjustement *)
-
-Theorem bir_get_stmt_bir_spinlockfull_prog_BirStmt_Generic =
-  EVAL ``bir_get_stmt bir_spinlockfull_prog x = BirStmt_Generic stm``
-  |> SIMP_RULE (srw_ss() ++ boolSimps.DNF_ss) [AllCaseEqs(),wordsTheory.NUMERAL_LESS_THM]
-  |> SIMP_RULE (srw_ss() ++ boolSimps.CONJ_ss) []
-  |> GEN_ALL
-
-Theorem bir_get_stmt_bir_spinlockfull_prog_BirStmt_Fence =
-  EVAL ``bir_get_stmt bir_spinlockfull_prog x = BirStmt_Fence mo1 mo2``
-  |> SIMP_RULE (srw_ss() ++ boolSimps.DNF_ss) [AllCaseEqs(),wordsTheory.NUMERAL_LESS_THM]
-  |> SIMP_RULE (srw_ss() ++ boolSimps.CONJ_ss) []
-  |> GEN_ALL
-
-Theorem bir_get_stmt_bir_spinlockfull_prog_BirStmt_Branch =
-  EVAL ``bir_get_stmt bir_spinlockfull_prog x = BirStmt_Branch a1 a2 a3``
-  |> SIMP_RULE (srw_ss() ++ boolSimps.DNF_ss) [AllCaseEqs(),wordsTheory.NUMERAL_LESS_THM]
-  |> SIMP_RULE (srw_ss() ++ boolSimps.CONJ_ss) []
-  |> GEN_ALL
-
-Theorem bir_get_stmt_bir_spinlockfull_prog_BirStmt_Expr =
-  EVAL ``bir_get_stmt bir_spinlockfull_prog x = BirStmt_Expr var e``
-  |> SIMP_RULE (srw_ss() ++ boolSimps.DNF_ss) [AllCaseEqs(),wordsTheory.NUMERAL_LESS_THM]
-  |> SIMP_RULE (srw_ss() ++ boolSimps.CONJ_ss) []
-  |> CONV_RULE $ ONCE_DEPTH_CONV $ RHS_CONV $ computeLib.EVAL_CONV
-  |> GEN_ALL
-
-(*
-Theorem bir_get_stmt_bir_spinlockfull_prog_BirStmt_Amo =
-  EVAL ``bir_get_stmt bir_spinlockfull_prog x = BirStmt_Amo var a_e v_e acq rel``
-  |> SIMP_RULE (srw_ss() ++ boolSimps.DNF_ss) [AllCaseEqs()]
-  |> GEN_ALL
-*)
-
-Theorem bir_get_stmt_bir_spinlockfull_prog_BirStmt_None =
-  EVAL ``bir_get_stmt bir_spinlockfull_prog x = BirStmt_None``
-  |> SIMP_RULE (srw_ss() ++ boolSimps.DNF_ss) [AllCaseEqs(),wordsTheory.NUMERAL_LESS_THM]
-  |> SIMP_RULE (srw_ss() ++ boolSimps.CONJ_ss) [AC CONJ_ASSOC CONJ_COMM]
-  |> GEN_ALL
-
-(* TODO calculate is_rel_def,is_amo_def,is_xcl_read_def,is_acq_def *)
-Theorem bir_get_stmt_bir_spinlockfull_prog_BirStmt_Read =
-  REFL ``bir_get_stmt bir_spinlockfull_prog pc = BirStmt_Read var a_e opt_cast xcl acq rel``
-  |> CONV_RULE $ DEPTH_CONV $ RHS_CONV $ REWRITE_CONV [bir_get_stmt_write,bir_get_stmt_read]
-  |> CONV_RULE $ DEPTH_CONV $ RHS_CONV $ ONCE_DEPTH_CONV $ REWRITE_CONV [Once bir_spinlockfull_prog_def]
-  |> SIMP_RULE (srw_ss() ++ boolSimps.DNF_ss) [bir_programTheory.bir_get_program_block_info_by_label_THM,pairTheory.LAMBDA_PROD,wordsTheory.NUMERAL_LESS_THM,bir_programTheory.bir_get_current_statement_def,CaseEq"option"]
-  |> SIMP_RULE (srw_ss() ++ boolSimps.CONJ_ss) [GSYM pairTheory.PEXISTS_THM]
-  |> SIMP_RULE (srw_ss() ++ boolSimps.DNF_ss ++ boolSimps.CONJ_ss) [bir_program_labelsTheory.BL_Address_HC_def]
-  |> SIMP_RULE (bool_ss ++ boolSimps.COND_elim_ss ++ boolSimps.DNF_ss ++ boolSimps.CONJ_ss) []
-  |> SIMP_RULE (srw_ss()) []
-  |> SIMP_RULE (bool_ss ++ boolSimps.DNF_ss) [EL,wordsTheory.NUMERAL_LESS_THM]
-  |> SIMP_RULE (srw_ss() ++ boolSimps.CONJ_ss ++ boolSimps.DNF_ss) [EL,get_read_args_def]
-  |> SIMP_RULE (bool_ss ++ boolSimps.DNF_ss) [EL,wordsTheory.NUMERAL_LESS_THM]
-  |> SIMP_RULE (srw_ss() ++ boolSimps.CONJ_ss ++ boolSimps.DNF_ss) [EL,get_read_args_def]
-  |> SIMP_RULE (bool_ss ++ boolSimps.DNF_ss) [EL,wordsTheory.NUMERAL_LESS_THM]
-  |> SIMP_RULE (srw_ss() ++ boolSimps.CONJ_ss ++ boolSimps.DNF_ss) [EL,get_read_args_def]
-
-(* TODO calculate is_rel_def,is_amo_def,is_xcl_write_def,is_acq_def *)
-Theorem bir_get_stmt_bir_spinlockfull_prog_BirStmt_Write =
-  REFL ``bir_get_stmt bir_spinlockfull_prog pc = BirStmt_Write a_e v_e xcl acq rel``
-  |> CONV_RULE $ DEPTH_CONV $ RHS_CONV $ REWRITE_CONV [bir_get_stmt_write,bir_get_stmt_read]
-  |> CONV_RULE $ DEPTH_CONV $ RHS_CONV $ ONCE_DEPTH_CONV $ REWRITE_CONV [Once bir_spinlockfull_prog_def]
-  |> SIMP_RULE (srw_ss() ++ boolSimps.DNF_ss) [bir_programTheory.bir_get_program_block_info_by_label_THM,pairTheory.LAMBDA_PROD,wordsTheory.NUMERAL_LESS_THM,bir_programTheory.bir_get_current_statement_def,CaseEq"option"]
-  |> SIMP_RULE (srw_ss() ++ boolSimps.CONJ_ss) [GSYM pairTheory.PEXISTS_THM]
-  |> SIMP_RULE (srw_ss() ++ boolSimps.DNF_ss ++ boolSimps.CONJ_ss) [bir_program_labelsTheory.BL_Address_HC_def]
-  |> SIMP_RULE (bool_ss ++ boolSimps.COND_elim_ss ++ boolSimps.DNF_ss ++ boolSimps.CONJ_ss) []
-  |> SIMP_RULE (srw_ss()) []
-  |> SIMP_RULE (bool_ss ++ boolSimps.DNF_ss) [EL,wordsTheory.NUMERAL_LESS_THM]
-  |> SIMP_RULE (srw_ss() ++ boolSimps.CONJ_ss ++ boolSimps.DNF_ss) [EL,get_fulfil_args_def,get_read_args_def]
-  |> SIMP_RULE (bool_ss ++ boolSimps.DNF_ss) [EL,wordsTheory.NUMERAL_LESS_THM]
-  |> SIMP_RULE (srw_ss() ++ boolSimps.CONJ_ss ++ boolSimps.DNF_ss) [EL,get_fulfil_args_def,get_read_args_def]
-  |> SIMP_RULE (bool_ss ++ boolSimps.DNF_ss) [EL,wordsTheory.NUMERAL_LESS_THM]
-  |> SIMP_RULE (srw_ss() ++ boolSimps.CONJ_ss ++ boolSimps.DNF_ss) [EL,get_fulfil_args_def,get_read_args_def]
-  |> SIMP_RULE (bool_ss ++ boolSimps.DNF_ss) [EL,wordsTheory.NUMERAL_LESS_THM]
-  |> SIMP_RULE (srw_ss() ++ boolSimps.CONJ_ss ++ boolSimps.DNF_ss) [EL,get_fulfil_args_def,get_read_args_def]
-  |> SIMP_RULE (bool_ss ++ boolSimps.DNF_ss) [EL,wordsTheory.NUMERAL_LESS_THM]
-  |> SIMP_RULE (srw_ss() ++ boolSimps.CONJ_ss ++ boolSimps.DNF_ss) [EL,get_fulfil_args_def,get_read_args_def]
-
-(* all possible steps of the full spinlock
- * sl_step (block,pc) (block',pc') *)
-(* TODO automate *)
-
-Inductive slf_step:
-     slf_step (BL_Address $ Imm64 0w,0n) (BL_Address $ Imm64 4w,0n)
-  /\ slf_step (BL_Address $ Imm64 4w,0)  (BL_Address $ Imm64 8w,0)
-  /\ slf_step (BL_Address $ Imm64 8w,0)  (BL_Address $ Imm64 4w,0)
-  /\ slf_step (BL_Address $ Imm64 8w,0)  (BL_Address $ Imm64 12w,0)
-  /\ slf_step (BL_Address $ Imm64 12w,0) (BL_Address $ Imm64 16w,0)
-  /\ slf_step (BL_Address $ Imm64 16w,0) (BL_Address $ Imm64 20w,0)
-  /\ slf_step (BL_Address $ Imm64 20w,0) (BL_Address $ Imm64 4w,0)
-  /\ slf_step (BL_Address $ Imm64 20w,0) (BL_Address $ Imm64 24w,0)
-  /\ slf_step (BL_Address $ Imm64 24w,0) (BL_Address $ Imm64 28w,0)
-  /\ slf_step (BL_Address $ Imm64 28w,0) (BL_Address $ Imm64 32w,0)
-  /\ slf_step (BL_Address $ Imm64 32w,0) (BL_Address $ Imm64 36w,0)
-  /\ slf_step (BL_Address $ Imm64 36w,0) (BL_Address $ Imm64 40w,0)
-End
-
-(* pc is reachable for bir_spinlockfull_prog from its first pc *)
-(* TODO automate *)
-
-Definition reachable_slf_def:
-  reachable_slf pc =
-    !bpt. bpt = bst_pc_tuple pc ==>
-         bpt = (BL_Address $ Imm64 0w,0n) \/ bpt = (BL_Address $ Imm64 4w,0)
-      \/ bpt = (BL_Address $ Imm64 8w,0)  \/ bpt = (BL_Address $ Imm64 12w,0)
-      \/ bpt = (BL_Address $ Imm64 16w,0) \/ bpt = (BL_Address $ Imm64 20w,0)
-      \/ bpt = (BL_Address $ Imm64 24w,0) \/ bpt = (BL_Address $ Imm64 28w,0)
-      \/ bpt = (BL_Address $ Imm64 32w,0) \/ bpt = (BL_Address $ Imm64 36w,0)
-      \/ bpt = (BL_Address $ Imm64 40w,0)
-End
-
-(* pc within crit region *)
-
-Definition in_crit_slf_def:
-  in_crit_slf pc <=>
-    reachable_asl pc /\ bst_pc_tuple pc = (BL_Address $ Imm64 32w,0)
-End
-
-(* pc not in lock or unlock region *)
-Definition outside_un_lock_slf_def:
-  outside_un_lock_slf pc <=>
-    !x n. bst_pc_tuple pc = (BL_Address $ Imm64 x,n)
-    ==>  (x,n) = (0w,0)
-      \/ (24w <= x /\ x <= 36w)
-      \/ x = 40w
-End
-
-(* thread  cid  sees a free lock *)
-
-Definition is_free_slf_def:
-  is_free_slf cid S <=>
-    bir_read_mem_var "MEM8" "x7" ((core_state cid S).bst_environ)
-    = SOME $ BVal_Imm $ Imm64 0w
-End
-
-(*****************************************************************************)
-(* Spinlock specification ****************************************************)
-(*****************************************************************************)
-
-(* returns the word with the cid's bit set to 1
-0...010...0 : word64
-     ^
-    cid
-
-requires cid < 64 *)
-
-Definition cid2w_def:
-  cid2w (cid : num) =
-    (* left shift of 1 by cid *)
-    BExp_BinExp BIExp_LeftShift (BExp_Const $ Imm64 1w) (BExp_Const $ Imm64 $ (n2w cid) :word64)
-End
-
-(* Abstract spinlock specification that is parametrised by its core id.
- * The core id is used to mark the lock as taken.
- * Requires a limited number of threads (inherited by cid2w) *)
-
-Definition spinlock_aprog_def:
-  spinlock_aprog cid =
-  BirProgram [
-  (* lock block *)
-  <|bb_label := BL_Address_HC (Imm64 0w) "";
-    bb_mc_tags := SOME <|mc_atomic := T; mc_acq := F; mc_rel := F|>;
-    bb_statements :=
-      [
-        (* _tmp := _GHOST.crit *)
-        BStmt_Assign (BVar "_tmp" $ BType_Imm Bit64)
-          (* BExp_Load mem_e a_e endianness type *)
-            $ BExp_Load (BExp_Den $ BVar "_GHOST" $ BType_Mem Bit64 Bit8)
-                      (BExp_Den $ BVar "crit" $ BType_Imm Bit64)
-                      BEnd_LittleEndian Bit32;
-        (* _is_locked := (_tmp != 0) *)
-        BStmt_Assign (BVar "_is_locked" $ BType_Imm Bit64)
-          $ BExp_IfThenElse
-              (BExp_BinExp BIExp_And
-                (BExp_Const $ Imm64 0w)
-                (BExp_Den $ BVar "_tmp" $ BType_Imm Bit64))
-              (BExp_Const $ Imm64 1w)
-              (BExp_Const $ Imm64 0w);
-        (* lock if possible *)
-        BStmt_Assign (BVar "_ignore" $ BType_Imm Bit64)
-          $ BExp_Store (BExp_Den $ BVar "_GHOST" $ BType_Mem Bit64 Bit8)
-            (BExp_Den $ BVar "crit" $ BType_Imm Bit64)
-            BEnd_LittleEndian
-            $ BExp_IfThenElse
-                (BExp_Den $ BVar "_is_locked" $ BType_Imm Bit64)
-                (BExp_Den $ BVar "_tmp" $ BType_Imm Bit64)
-                (cid2w cid);
-      ];
-    (* spin on _is_locked *)
-    bb_last_statement :=
-        BStmt_CJmp
-          (BExp_Den $ BVar "_is_locked" $ BType_Imm Bit64)
-          (BLE_Label $ BL_Address $ Imm64 0w)
-          (BLE_Label $ BL_Address $ Imm64 4w);
-  |>;
-  (* unlock *)
-  <|bb_label := BL_Address_HC (Imm64 4w) "";
-    bb_mc_tags := SOME <|mc_atomic := F; mc_acq := F; mc_rel := F|>;
-    bb_statements :=
-      [
-(*
-reset lock availability for cid by writing
-_GHOST.crit := (1...101...1   AND   _GHOST.crit)
-                     ^
-                    cid
-*)
-      BStmt_Assign
-        (BVar "_GHOST" $ BType_Mem Bit64 Bit8)
-        $ BExp_Store (BExp_Den $ BVar "_GHOST" $ BType_Mem Bit64 Bit8)
-          (BExp_Den $ BVar "crit" $ BType_Imm Bit64)
-          BEnd_LittleEndian
-          $ BExp_BinExp BIExp_And
-              (BExp_Load (BExp_Den $ BVar "_GHOST" $ BType_Mem Bit64 Bit8)
-                (BExp_Den $ BVar "crit" $ BType_Imm Bit64)
-                BEnd_LittleEndian Bit32)
-              $ BExp_UnaryExp BIExp_Not $ cid2w cid;
-      ];
-    bb_last_statement := BStmt_Jmp $ BLE_Label $ BL_Address $ Imm64 8w
-  |>
-  ] : string bir_program_t
-End
-
-(* lookup _GHOST.crit to contain only zeros (= lock is free) *)
-(* TODO assume for initial state *)
-
-Definition is_free_asl_def:
-  is_free_asl g_env <=>
-    bir_read_mem_var "_GHOST" "crit" g_env = SOME $ BVal_Imm $ Imm64 0w
-End
-
-(* all possible steps of the abstract spinlock
- * sl_step (block,pc) (block',pc') *)
-(* TODO rename control flow *)
-(* TODO automate *)
-
-Inductive asl_step:
-     asl_step (BL_Address $ Imm64 0w,0n) (BL_Address $ Imm64 0w,1n)
-  /\ asl_step (BL_Address $ Imm64 0w,1)  (BL_Address $ Imm64 0w,2)
-  /\ asl_step (BL_Address $ Imm64 0w,2)  (BL_Address $ Imm64 0w,0)
-  /\ asl_step (BL_Address $ Imm64 0w,2)  (BL_Address $ Imm64 4w,0)
-  /\ asl_step (BL_Address $ Imm64 4w,0)  (BL_Address $ Imm64 8w,0)
-End
-
-(* pc is reachable for bir_spinlock from its first pc *)
-(* TODO automate *)
-
-Definition reachable_asl_def:
-  reachable_asl pc =
-    !bpt. bpt = bst_pc_tuple pc ==>
-    bpt = (BL_Address $ Imm64 0w,0) \/ bpt = (BL_Address $ Imm64 0w,1) \/
-    bpt = (BL_Address $ Imm64 0w,2) \/ bpt = (BL_Address $ Imm64 4w,0) \/
-    bpt = (BL_Address $ Imm64 8w,0)
-End
-
-(* pc within crit region *)
-(* the abstract program contains only one statement, thus behaves atomically *)
-Definition in_crit_asl_def:
-  in_crit_asl pc <=> reachable_asl pc
-End
-
-(* pc not in lock or unlock region *)
-Definition outside_un_lock_asl_def:
-  outside_un_lock_asl pc <=>
-    !x n. bst_pc_tuple pc = (BL_Address $ Imm64 x,n)
-    ==>  (x,n) = (0w,0)
-      \/ (x,n) = (4w,0)
-      \/ (x,n) = (8w,0)
-End
 
 (* TODO define statement *)
 Definition same_pc_als_slf_def:
   same_pc_als_slf pc pc' <=>
+(* manually match pcs in lock and unlock region *)
+(*
+  for abstract and concrete pc, project
+    (b,n) ∈ block x statement
+  into :num as
+    sum [i < b. blockwidth i]  + n
+  and equate (assuming the offset is accounted for)
+*)
     (ARB :bool)
 End
 
@@ -376,58 +26,246 @@ End
 (* TODO parametrise over projection of aS and S at cid *)
 Definition asl_slf_rel_def:
   asl_slf_rel cid aS S =
-  (!cores M acores aM agenv genv.
+  (!cores M acores aM agenv genv apc pc lbl index albl aindex.
        cores = FST S
     /\ M = FST $ SND S
     /\ genv = SND $ SND S
+    /\ pc = core_pc cid S
+    /\ lbl = core_pc_lbl cid S
+    /\ index = core_pc_index cid S
     /\ acores = FST aS
     /\ aM = FST $ SND aS
     /\ agenv = SND $ SND aS
+    /\ apc = core_pc cid aS
+    /\ albl = core_pc_lbl cid aS
+    /\ aindex = core_pc_index cid aS
     ==>
     (* we only reason about reachable states *)
-       reachable_asl (core_pc cid aS)
-    /\ reachable_slf (core_pc cid S)
+       reachable_asl apc
+    /\ reachable_slf pc
     /\ core_prog cid aS = spinlock_aprog cid
-    /\ core_prog cid S = bir_spinlockfull_prog
+    /\ core_prog cid S = (bir_spinlockfull_prog: string bir_program_t)
     (* lock is free *)
     /\ is_free_slf cid S = is_free_asl agenv
     (* pc outside lock and unlock *)
     /\ (
-      outside_un_lock_asl (core_pc cid aS)
-      /\ outside_un_lock_slf (core_pc cid S)
-      ==> same_pc_als_slf (core_pc cid aS) (core_pc cid S)
+      outside_un_lock_asl apc
+      /\ outside_un_lock_slf pc
+      ==> same_pc_als_slf apc pc
+(*
+spinlock_aprog_def
+bir_spinlockfull_prog_def
+*)
     )
     (* not taking the lock *)
     /\ (
-      (bir_laImm64_lt (FST $ bst_pc_tuple $ core_pc cid S) 20w
-      /\ (FST $ bst_pc_tuple $ core_pc cid S = BL_Address $ Imm64 20w ==>
+      (lbl < 20w
+      /\ (lbl = 20w ==>
           bir_read_core_reg_zero "x6" cid S) (* unsuccessful store *)
       ) ==> bst_pc_tuple $ core_pc cid aS = (BL_Address $ Imm64 0w,0)
     )
     (* future successful store *)
     /\ (
-        FST $ bst_pc_tuple $ core_pc cid S = BL_Address $ Imm64 20w
+        lbl = 20w
         /\ ~bir_read_core_reg_zero "x6" cid S
         ==> bst_pc_tuple $ core_pc cid aS = (BL_Address $ Imm64 4w,0)
     )
     (* successful store *)
     /\ (
-        FST $ bst_pc_tuple $ core_pc cid S = BL_Address $ Imm64 24w
+        lbl = 24w
         ==> bst_pc_tuple $ core_pc cid aS = (BL_Address $ Imm64 4w,0)
     )
     (* after lock, before unlock *)
     /\ (
-        bir_laImm64_lt2 24w (FST $ bst_pc_tuple $ core_pc cid S)
-        /\ bir_laImm64_lt (FST $ bst_pc_tuple $ core_pc cid S) 40w
+        24w < lbl /\ lbl < 40w
         ==> bst_pc_tuple $ core_pc cid aS = (BL_Address $ Imm64 4w,0)
     )
     (* after unlock *)
     /\ (
-        FST $ bst_pc_tuple $ core_pc cid S = BL_Address $ Imm64 40w
+        lbl = 40w
         ==> bst_pc_tuple $ core_pc cid aS = (BL_Address $ Imm64 8w,0)
     )
   )
 End
+
+
+(*****************************************************************************)
+(* The refinemen theorem(s) **************************************************)
+(*****************************************************************************)
+
+Theorem bir_spinlockfull_prog_not_is_xcl_write:
+  pc.bpc_label = BL_Address (Imm64 36w)
+  /\ pc.bpc_index = 2
+  ==> ~is_xcl_write bir_spinlockfull_prog pc
+Proof
+  rpt gen_tac >> strip_tac
+  >> EVAL_TAC
+  >> fs[]
+QED
+
+Theorem bir_spinlockfull_prog_is_xcl_write:
+  pc.bpc_label = BL_Address (Imm64 16w)
+  /\ pc.bpc_index = 2
+  ==> is_xcl_write bir_spinlockfull_prog pc
+Proof
+  rpt strip_tac
+  >> EVAL_TAC
+  >> fs[]
+QED
+
+Theorem bir_spinlockfull_prog_is_xcl_read:
+  pc.bpc_label = BL_Address (Imm64 4w)
+  /\ pc.bpc_index = 1
+  ==> is_xcl_read bir_spinlockfull_prog pc
+    $ BExp_Den $ BVar "x7" $ BType_Imm Bit64
+Proof
+  rpt strip_tac
+  >> EVAL_TAC
+  >> fs[]
+QED
+
+(* read transitions *)
+Theorem spinlock_refinement_Read:
+  !cid tr i aS st var a_e opt_cast xcl acq rel.
+  wf_trace tr /\ SUC i < LENGTH tr
+  /\ parstep_nice cid (EL i tr) (EL (SUC i) tr)
+  /\ asl_slf_rel cid aS (EL i tr)
+  /\ FLOOKUP (FST (EL i tr)) cid = SOME (Core cid (bir_spinlockfull_prog :string bir_program_t) st)
+  /\ FLOOKUP (FST aS) cid = SOME $ Core cid (spinlock_aprog cid) st'
+  /\ bir_get_stmt (bir_spinlockfull_prog :string bir_program_t) st.bst_pc =
+        BirStmt_Read var a_e opt_cast xcl acq rel
+  /\ FST (SND (EL i tr)) = FST (SND (EL (SUC i) tr))
+  ==>
+    asl_slf_rel cid aS (EL (SUC i) tr)
+    \/ ?aS'. parstep_nice cid aS aS'
+          /\ asl_slf_rel cid aS' (EL (SUC i) tr)
+Proof
+  rpt strip_tac
+  >> disj1_tac
+  >> drule_then strip_assume_tac $ iffLR bir_get_stmt_bir_spinlockfull_prog_BirStmt_Read
+  >> dxrule_then assume_tac $ iffLR parstep_nice_def
+  >> gs[parstep_cases,cstep_cases,clstep_cases,get_core_state_def,FLOOKUP_UPDATE,core_zoo,asl_slf_rel_def,bir_spinlockfull_prog_is_xcl_read,bir_programTheory.bir_pc_next_def,get_core_prog_def]
+  >> conj_tac
+  >- simp[reachable_slf_def,bst_pc_tuple_def]
+  >> conj_tac
+  >- (
+    qmatch_goalsub_abbrev_tac `_ = B`
+    >> qpat_x_assum `_ = B` $ fs o single o GSYM
+    >> fs[is_free_slf_def,core_zoo,bir_read_mem_var_def,FLOOKUP_UPDATE]
+    (* MEM8.x7 holds the default 0w before and after reading from *)
+    >> qpat_x_assum `_ = bir_eval_exp_view _ _ _ _` mp_tac
+    >> fs[bir_eval_exp_view_def,bir_eval_exp_mix_def,is_global_def]
+    >> fs[]
+    >> cheat
+  )
+  >> cheat
+QED
+
+(* write transitions *)
+Theorem spinlock_refinement_Write:
+  !cid tr i aS st a_e v_e xcl acq rel.
+  wf_trace tr /\ SUC i < LENGTH tr
+  /\ parstep_nice cid (EL i tr) (EL (SUC i) tr)
+  /\ asl_slf_rel cid aS (EL i tr)
+  /\ FLOOKUP (FST (EL i tr)) cid = SOME (Core cid bir_spinlockfull_prog st)
+  /\ bir_get_stmt bir_spinlockfull_prog st.bst_pc =
+    BirStmt_Write a_e v_e xcl acq rel
+  /\ FST (SND (EL i tr)) = FST (SND (EL (SUC i) tr))
+  ==>
+    asl_slf_rel cid aS (EL (SUC i) tr)
+    \/ ?aS'. parstep_nice cid aS aS'
+          /\ asl_slf_rel cid aS' (EL (SUC i) tr)
+Proof
+  cheat
+QED
+
+(* generic transitions *)
+Theorem spinlock_refinement_Generic:
+  !cid tr i aS st stm.
+  wf_trace tr /\ SUC i < LENGTH tr
+  /\ parstep_nice cid (EL i tr) (EL (SUC i) tr)
+  /\ asl_slf_rel cid aS (EL i tr)
+  /\ FLOOKUP (FST (EL i tr)) cid = SOME (Core cid bir_spinlockfull_prog st)
+  /\ bir_get_stmt bir_spinlockfull_prog st.bst_pc = BirStmt_Generic stm
+  /\ FST (SND (EL i tr)) = FST (SND (EL (SUC i) tr))
+  ==>
+    asl_slf_rel cid aS (EL (SUC i) tr)
+    \/ ?aS'. parstep_nice cid aS aS'
+          /\ asl_slf_rel cid aS' (EL (SUC i) tr)
+Proof
+  cheat
+QED
+
+(* fence transitions *)
+Theorem spinlock_refinement_Fence:
+  !cid tr i aS st mo1 mo2.
+  wf_trace tr /\ SUC i < LENGTH tr
+  /\ parstep_nice cid (EL i tr) (EL (SUC i) tr)
+  /\ asl_slf_rel cid aS (EL i tr)
+  /\ FLOOKUP (FST (EL i tr)) cid = SOME (Core cid bir_spinlockfull_prog st)
+  /\ bir_get_stmt (bir_spinlockfull_prog :string bir_program_t) st.bst_pc = BirStmt_Fence mo1 mo2
+  /\ FST (SND (EL i tr)) = FST (SND (EL (SUC i) tr))
+  ==>
+    asl_slf_rel cid aS (EL (SUC i) tr)
+    \/ ?aS'. parstep_nice cid aS aS'
+          /\ asl_slf_rel cid aS' (EL (SUC i) tr)
+Proof
+  cheat
+QED
+
+(* expr transitions *)
+Theorem spinlock_refinement_Expr:
+  !cid tr i aS st var e.
+  wf_trace tr /\ SUC i < LENGTH tr
+  /\ parstep_nice cid (EL i tr) (EL (SUC i) tr)
+  /\ asl_slf_rel cid aS (EL i tr)
+  /\ FLOOKUP (FST (EL i tr)) cid = SOME (Core cid bir_spinlockfull_prog st)
+  /\ bir_get_stmt bir_spinlockfull_prog st.bst_pc = BirStmt_Expr var e
+  /\ FST (SND (EL i tr)) = FST (SND (EL (SUC i) tr))
+  ==>
+    asl_slf_rel cid aS (EL (SUC i) tr)
+    \/ ?aS'. parstep_nice cid aS aS'
+          /\ asl_slf_rel cid aS' (EL (SUC i) tr)
+Proof
+  cheat
+QED
+
+(* branch transitions *)
+Theorem spinlock_refinement_Branch:
+  !cid tr i aS st a1 a2 a3.
+  wf_trace tr /\ SUC i < LENGTH tr
+  /\ parstep_nice cid (EL i tr) (EL (SUC i) tr)
+  /\ asl_slf_rel cid aS (EL i tr)
+  /\ FLOOKUP (FST (EL i tr)) cid = SOME (Core cid bir_spinlockfull_prog st)
+  /\ bir_get_stmt bir_spinlockfull_prog st.bst_pc = BirStmt_Branch a1 a2 a3
+  /\ FST (SND (EL i tr)) = FST (SND (EL (SUC i) tr))
+  ==>
+    asl_slf_rel cid aS (EL (SUC i) tr)
+    \/ ?aS'. parstep_nice cid aS aS'
+          /\ asl_slf_rel cid aS' (EL (SUC i) tr)
+Proof
+  cheat
+QED
+
+(* amo transitions *)
+(* TODO no amo instructions;
+   solved by evaluating bir_get_stmt_bir_spinlockfull_prog_BirStmt_Amo *)
+Theorem spinlock_refinement_Amo:
+  !cid tr i aS st var a_e v_e acq rel.
+  wf_trace tr /\ SUC i < LENGTH tr
+  /\ parstep_nice cid (EL i tr) (EL (SUC i) tr)
+  /\ asl_slf_rel cid aS (EL i tr)
+  /\ FLOOKUP (FST (EL i tr)) cid = SOME (Core cid bir_spinlockfull_prog st)
+  /\ bir_get_stmt bir_spinlockfull_prog st.bst_pc =
+    BirStmt_Amo var a_e v_e acq rel
+  /\ FST (SND (EL i tr)) = FST (SND (EL (SUC i) tr))
+  ==>
+    asl_slf_rel cid aS (EL (SUC i) tr)
+    \/ ?aS'. parstep_nice cid aS aS'
+          /\ asl_slf_rel cid aS' (EL (SUC i) tr)
+Proof
+  cheat
+QED
 
 (* refinement theorem *)
 (* the abstract state is prefixed with "a" *)
@@ -442,8 +280,80 @@ Theorem spinlock_refinement:
     \/ ?aS'. parstep_nice cid aS aS'
           /\ asl_slf_rel cid aS' (EL (SUC i) tr)
 Proof
-  cheat
+  rpt strip_tac
+  >> drule_then assume_tac $ iffLR asl_slf_rel_def
+  >> gs[]
+  >> reverse $ drule_then strip_assume_tac parstep_nice_memory_imp
+  (* promise case *)
+  >- (
+    disj1_tac
+    >> cheat (* no relevant change of state *)
+  )
+  >> qmatch_asmsub_rename_tac `asl_slf_rel cid aS' _`
+  >> `?st st' ast.
+    FLOOKUP (FST (EL i tr)) cid = SOME (Core cid (bir_spinlockfull_prog :string bir_program_t) st)
+    /\ FLOOKUP (FST (EL (SUC i) tr)) cid = SOME (Core cid (bir_spinlockfull_prog :string bir_program_t) st')
+    /\ FLOOKUP (FST aS') cid = SOME (Core cid (spinlock_aprog cid) ast)
+  ` by (
+    cheat
+  )
+  >> gvs[core_pc_def,core_state_def,get_core_state_def,core_def,parstep_nice_def,bst_pc_tuple_def,core_pc_lbl_def,core_pc_index_def,addr_val_def]
+  >> drule_then strip_assume_tac $ iffLR parstep_cases
+  >> gs[clstep_cases,cstep_cases]
+  (* 8 goals *)
+  >~ [`bir_get_stmt _ _ = BirStmt_Write a_e v_e xcl acq rel`]
+  >- (
+    drule_at (Pat `bir_get_stmt _ _ = _`) spinlock_refinement_Write
+    >> rpt $ disch_then $ drule_at Any
+    >> fs[parstep_nice_def]
+  )
+  >~ [`bir_get_stmt _ _ = BirStmt_Write a_e v_e xcl acq rel`]
+  >- (
+    drule_at (Pat `bir_get_stmt _ _ = _`) spinlock_refinement_Write
+    >> rpt $ disch_then $ drule_at Any
+    >> fs[parstep_nice_def]
+  )
+  >~ [`bir_get_stmt _ _ = BirStmt_Read var a_e opt_cast xcl acq rel`]
+  >- (
+    drule_at (Pat `bir_get_stmt _ _ = _`) spinlock_refinement_Read
+    >> rpt $ disch_then $ drule_at Any
+    >> fs[parstep_nice_def]
+  )
+  >~ [`bir_get_stmt _ _ = BirStmt_Fence mo1 mo2`]
+  >- (
+    drule_at (Pat `bir_get_stmt _ _ = _`) spinlock_refinement_Fence
+    >> rpt $ disch_then $ drule_at Any
+    >> fs[parstep_nice_def]
+  )
+  >~ [`bir_get_stmt _ _ = BirStmt_Generic stm`]
+  >- (
+    drule_at (Pat `bir_get_stmt _ _ = _`) spinlock_refinement_Generic
+    >> rpt $ disch_then $ drule_at Any
+    >> fs[parstep_nice_def]
+  )
+  >~ [`bir_get_stmt _ _ = BirStmt_Branch a1 a2 a3`]
+  >- (
+    drule_at (Pat `bir_get_stmt _ _ = _`) spinlock_refinement_Branch
+    >> rpt $ disch_then $ drule_at Any
+    >> fs[parstep_nice_def]
+  )
+  >~ [`bir_get_stmt _ _ = BirStmt_Amo var a_e v_e acq rel`]
+  >- (
+    drule_at (Pat `bir_get_stmt _ _ = _`) spinlock_refinement_Amo
+    >> rpt $ disch_then $ drule_at Any
+    >> fs[parstep_nice_def]
+  )
+  >~ [`bir_get_stmt _ _ = BirStmt_Expr var e`]
+  >- (
+    drule_at (Pat `bir_get_stmt _ _ = _`) spinlock_refinement_Expr
+    >> rpt $ disch_then $ drule_at Any
+    >> fs[parstep_nice_def]
+  )
 QED
+
+(*
+reachability for free for traces
+*)
 
 val _ = export_theory();
 
