examples/spinlock/spinlockAbstractScript.sml
@@ -1,0 +1,265 @@
+open HolKernel Parse boolLib bossLib;
+open rich_listTheory listTheory arithmeticTheory finite_mapTheory ;
+open bir_lifter_interfaceLib ;
+open bir_promisingTheory ;
+open tracesTheory ;
+(* TODO currently some general definitions are in spinlockConcreteTheory *)
+open spinlockConcreteTheory ;
+
+val _ = new_theory "spinlockAbstract";
+
+(*****************************************************************************)
+(* Spinlock specification ****************************************************)
+(*****************************************************************************)
+
+(* returns the word with the cid's bit set to 1
+0...010...0 : word64
+     ^
+    cid
+
+requires cid < 64 *)
+
+Definition cid2w_def:
+  cid2w (cid : num) =
+    (* left shift of 1 by cid *)
+    BExp_BinExp BIExp_LeftShift (BExp_Const $ Imm64 1w) (BExp_Const $ Imm64 $ (n2w cid) :word64)
+End
+
+(* Abstract spinlock specification that is parametrised by its core id.
+ * The core id is used to mark the lock as taken.
+ * Requires a limited number of threads (inherited by cid2w) *)
+
+Definition spinlock_aprog_def:
+  spinlock_aprog cid =
+  BirProgram [
+  (* lock block *)
+  <|bb_label := BL_Address_HC (Imm64 0w) "";
+    bb_mc_tags := SOME <|mc_atomic := T; mc_acq := F; mc_rel := F|>;
+    bb_statements :=
+      [
+        (* _tmp := _GHOST.crit *)
+        BStmt_Assign (BVar "_tmp" $ BType_Imm Bit64)
+          (* BExp_Load mem_e a_e endianness type *)
+            $ BExp_Load (BExp_Den $ BVar "_GHOST" $ BType_Mem Bit64 Bit8)
+                      (BExp_Den $ BVar "crit" $ BType_Imm Bit64)
+                      BEnd_LittleEndian Bit32;
+        (* _is_locked := (_tmp != 0) *)
+        BStmt_Assign (BVar "_is_locked" $ BType_Imm Bit64)
+          $ BExp_IfThenElse
+              (BExp_BinExp BIExp_And
+                (BExp_Const $ Imm64 0w)
+                (BExp_Den $ BVar "_tmp" $ BType_Imm Bit64))
+              (BExp_Const $ Imm64 1w)
+              (BExp_Const $ Imm64 0w);
+        (* lock if possible *)
+        BStmt_Assign (BVar "_ignore" $ BType_Imm Bit64)
+          $ BExp_Store (BExp_Den $ BVar "_GHOST" $ BType_Mem Bit64 Bit8)
+            (BExp_Den $ BVar "crit" $ BType_Imm Bit64)
+            BEnd_LittleEndian
+            $ BExp_IfThenElse
+                (BExp_Den $ BVar "_is_locked" $ BType_Imm Bit64)
+                (BExp_Den $ BVar "_tmp" $ BType_Imm Bit64)
+                (cid2w cid);
+      ];
+    (* spin on _is_locked *)
+    bb_last_statement :=
+        BStmt_CJmp
+          (BExp_Den $ BVar "_is_locked" $ BType_Imm Bit64)
+          (BLE_Label $ BL_Address $ Imm64 0w)
+          (BLE_Label $ BL_Address $ Imm64 4w);
+  |>;
+  (* unlock *)
+  <|bb_label := BL_Address_HC (Imm64 4w) "";
+    bb_mc_tags := SOME <|mc_atomic := F; mc_acq := F; mc_rel := F|>;
+    bb_statements :=
+      [
+(*
+reset lock availability for cid by writing
+_GHOST.crit := (1...101...1   AND   _GHOST.crit)
+                     ^
+                    cid
+*)
+      BStmt_Assign
+        (BVar "_GHOST" $ BType_Mem Bit64 Bit8)
+        $ BExp_Store (BExp_Den $ BVar "_GHOST" $ BType_Mem Bit64 Bit8)
+          (BExp_Den $ BVar "crit" $ BType_Imm Bit64)
+          BEnd_LittleEndian
+          $ BExp_BinExp BIExp_And
+              (BExp_Load (BExp_Den $ BVar "_GHOST" $ BType_Mem Bit64 Bit8)
+                (BExp_Den $ BVar "crit" $ BType_Imm Bit64)
+                BEnd_LittleEndian Bit32)
+              $ BExp_UnaryExp BIExp_Not $ cid2w cid;
+      ];
+    bb_last_statement := BStmt_Jmp $ BLE_Label $ BL_Address $ Imm64 8w
+  |>
+  ] : string bir_program_t
+End
+
+(* lookup _GHOST.crit to contain only zeros (= lock is free) *)
+(* TODO assume for initial state *)
+
+Definition is_free_asl_def:
+  is_free_asl g_env <=>
+    bir_read_mem_var "_GHOST" "crit" g_env = SOME $ BVal_Imm $ Imm64 0w
+End
+
+(*****************************************************************************)
+(* Extracting reachable states of a program **********************************)
+(*****************************************************************************)
+(* TODO some theorems need further adjustement *)
+
+Theorem bir_get_stmt_spinlock_aprog_BirStmt_Generic =
+  EVAL ``bir_get_stmt (spinlock_aprog cid) x = BirStmt_Generic stm``
+  |> SIMP_RULE (srw_ss() ++ boolSimps.DNF_ss) [AllCaseEqs(),wordsTheory.NUMERAL_LESS_THM]
+  |> SIMP_RULE (srw_ss() ++ boolSimps.CONJ_ss) []
+  |> GEN_ALL
+
+Theorem bir_get_stmt_spinlock_aprog_BirStmt_Fence =
+  EVAL ``bir_get_stmt (spinlock_aprog cid) x = BirStmt_Fence mo1 mo2``
+  |> SIMP_RULE (srw_ss() ++ boolSimps.DNF_ss) [AllCaseEqs(),wordsTheory.NUMERAL_LESS_THM]
+  |> SIMP_RULE (srw_ss() ++ boolSimps.CONJ_ss) []
+  |> GEN_ALL
+
+Theorem bir_get_stmt_spinlock_aprog_BirStmt_Branch =
+  EVAL ``bir_get_stmt (spinlock_aprog cid) x = BirStmt_Branch a1 a2 a3``
+  |> SIMP_RULE (srw_ss() ++ boolSimps.DNF_ss) [AllCaseEqs(),wordsTheory.NUMERAL_LESS_THM]
+  |> SIMP_RULE (srw_ss() ++ boolSimps.CONJ_ss) []
+  |> GEN_ALL
+
+Theorem bir_get_stmt_spinlock_aprog_BirStmt_Expr =
+  EVAL ``bir_get_stmt (spinlock_aprog cid) x = BirStmt_Expr var e``
+  |> SIMP_RULE (srw_ss() ++ boolSimps.DNF_ss) [AllCaseEqs(),wordsTheory.NUMERAL_LESS_THM]
+  |> SIMP_RULE (srw_ss() ++ boolSimps.CONJ_ss) []
+  |> CONV_RULE $ ONCE_DEPTH_CONV $ RHS_CONV $ computeLib.EVAL_CONV
+  |> GEN_ALL
+
+(*
+Theorem bir_get_stmt_spinlock_aprog_BirStmt_Amo =
+  EVAL ``bir_get_stmt (spinlock_aprog cid) x = BirStmt_Amo var a_e v_e acq rel``
+  |> SIMP_RULE (srw_ss() ++ boolSimps.DNF_ss) [AllCaseEqs()]
+  |> GEN_ALL
+*)
+
+Theorem bir_get_stmt_spinlock_aprog_BirStmt_Amo:
+  !x cid var a_e v_e acq rel.
+  bir_get_stmt (spinlock_aprog cid) x = BirStmt_Amo var a_e v_e acq rel ==> F
+Proof
+  cheat
+QED
+
+Theorem bir_get_stmt_spinlock_aprog_BirStmt_None =
+  EVAL ``bir_get_stmt (spinlock_aprog cid) x = BirStmt_None``
+  |> SIMP_RULE (srw_ss() ++ boolSimps.DNF_ss) [AllCaseEqs(),wordsTheory.NUMERAL_LESS_THM]
+  |> SIMP_RULE (srw_ss() ++ boolSimps.CONJ_ss) [AC CONJ_ASSOC CONJ_COMM]
+  |> SIMP_RULE (srw_ss() ++ boolSimps.DNF_ss) [get_read_args_def,get_fulfil_args_def]
+  |> GEN_ALL
+
+(* TODO calculate is_rel_def,is_amo_def,is_xcl_read_def,is_acq_def *)
+Theorem bir_get_stmt_spinlock_aprog_BirStmt_Read =
+  REFL ``bir_get_stmt (spinlock_aprog cid) pc = BirStmt_Read var a_e opt_cast xcl acq rel``
+  |> CONV_RULE $ DEPTH_CONV $ RHS_CONV $ REWRITE_CONV [bir_get_stmt_write,bir_get_stmt_read]
+  |> CONV_RULE $ DEPTH_CONV $ RHS_CONV $ ONCE_DEPTH_CONV $ REWRITE_CONV [Once spinlock_aprog_def]
+  |> SIMP_RULE (srw_ss() ++ boolSimps.DNF_ss) [bir_programTheory.bir_get_program_block_info_by_label_THM,pairTheory.LAMBDA_PROD,wordsTheory.NUMERAL_LESS_THM,bir_programTheory.bir_get_current_statement_def,CaseEq"option"]
+  |> SIMP_RULE (srw_ss() ++ boolSimps.CONJ_ss) [GSYM pairTheory.PEXISTS_THM]
+  |> SIMP_RULE (srw_ss() ++ boolSimps.DNF_ss ++ boolSimps.CONJ_ss) [bir_program_labelsTheory.BL_Address_HC_def]
+  |> SIMP_RULE (bool_ss ++ boolSimps.COND_elim_ss ++ boolSimps.DNF_ss ++ boolSimps.CONJ_ss) []
+  |> SIMP_RULE (srw_ss()) []
+  |> SIMP_RULE (bool_ss ++ boolSimps.DNF_ss) [EL,wordsTheory.NUMERAL_LESS_THM]
+  |> SIMP_RULE (srw_ss() ++ boolSimps.CONJ_ss ++ boolSimps.DNF_ss) [EL,get_read_args_def]
+  |> SIMP_RULE (bool_ss ++ boolSimps.DNF_ss) [EL,wordsTheory.NUMERAL_LESS_THM]
+  |> SIMP_RULE (srw_ss() ++ boolSimps.CONJ_ss ++ boolSimps.DNF_ss) [EL,get_read_args_def]
+  |> SIMP_RULE (bool_ss ++ boolSimps.DNF_ss) [EL,wordsTheory.NUMERAL_LESS_THM]
+  |> SIMP_RULE (srw_ss() ++ boolSimps.CONJ_ss ++ boolSimps.DNF_ss) [EL,get_read_args_def]
+
+(* TODO calculate is_rel_def,is_amo_def,is_xcl_write_def,is_acq_def *)
+Theorem bir_get_stmt_spinlock_aprog_BirStmt_Write =
+  REFL ``bir_get_stmt (spinlock_aprog cid) pc = BirStmt_Write a_e v_e xcl acq rel``
+  |> CONV_RULE $ DEPTH_CONV $ RHS_CONV $ REWRITE_CONV [bir_get_stmt_write,bir_get_stmt_read]
+  |> CONV_RULE $ DEPTH_CONV $ RHS_CONV $ ONCE_DEPTH_CONV $ REWRITE_CONV [Once spinlock_aprog_def]
+  |> SIMP_RULE (srw_ss() ++ boolSimps.DNF_ss) [bir_programTheory.bir_get_program_block_info_by_label_THM,pairTheory.LAMBDA_PROD,wordsTheory.NUMERAL_LESS_THM,bir_programTheory.bir_get_current_statement_def,CaseEq"option"]
+  |> SIMP_RULE (srw_ss() ++ boolSimps.CONJ_ss) [GSYM pairTheory.PEXISTS_THM]
+  |> SIMP_RULE (srw_ss() ++ boolSimps.DNF_ss ++ boolSimps.CONJ_ss) [bir_program_labelsTheory.BL_Address_HC_def]
+  |> SIMP_RULE (bool_ss ++ boolSimps.COND_elim_ss ++ boolSimps.DNF_ss ++ boolSimps.CONJ_ss) []
+  |> SIMP_RULE (srw_ss()) []
+  |> SIMP_RULE (bool_ss ++ boolSimps.DNF_ss) [EL,wordsTheory.NUMERAL_LESS_THM]
+  |> SIMP_RULE (srw_ss() ++ boolSimps.CONJ_ss ++ boolSimps.DNF_ss) [EL,get_fulfil_args_def,get_read_args_def]
+  |> SIMP_RULE (bool_ss ++ boolSimps.DNF_ss) [EL,wordsTheory.NUMERAL_LESS_THM]
+  |> SIMP_RULE (srw_ss() ++ boolSimps.CONJ_ss ++ boolSimps.DNF_ss) [EL,get_fulfil_args_def,get_read_args_def]
+  |> SIMP_RULE (bool_ss ++ boolSimps.DNF_ss) [EL,wordsTheory.NUMERAL_LESS_THM]
+  |> SIMP_RULE (srw_ss() ++ boolSimps.CONJ_ss ++ boolSimps.DNF_ss) [EL,get_fulfil_args_def,get_read_args_def]
+  |> SIMP_RULE (bool_ss ++ boolSimps.DNF_ss) [EL,wordsTheory.NUMERAL_LESS_THM]
+  |> SIMP_RULE (srw_ss() ++ boolSimps.CONJ_ss ++ boolSimps.DNF_ss) [EL,get_fulfil_args_def,get_read_args_def]
+  |> SIMP_RULE (bool_ss ++ boolSimps.DNF_ss) [EL,wordsTheory.NUMERAL_LESS_THM]
+  |> SIMP_RULE (srw_ss() ++ boolSimps.CONJ_ss ++ boolSimps.DNF_ss) [EL,get_fulfil_args_def,get_read_args_def]
+
+Theorem bir_get_stmt_spinlock_thms =
+  LIST_CONJ $
+  map (CONV_RULE (ONCE_DEPTH_CONV $ LHS_CONV SYM_CONV))
+    [bir_get_stmt_spinlock_aprog_BirStmt_Generic,
+    bir_get_stmt_spinlock_aprog_BirStmt_Fence,
+    bir_get_stmt_spinlock_aprog_BirStmt_Branch,
+    bir_get_stmt_spinlock_aprog_BirStmt_Expr,
+    bir_get_stmt_spinlock_aprog_BirStmt_None,
+    bir_get_stmt_spinlock_aprog_BirStmt_Amo,
+    bir_get_stmt_spinlock_aprog_BirStmt_Write,
+    bir_get_stmt_spinlock_aprog_BirStmt_Read]
+
+Theorem bir_spinlock_aprog_is_xcl_write:
+  !cid pc. pc.bpc_label = BL_Address (Imm64 0w) /\ pc.bpc_index = 0
+  ==>
+    ~is_xcl_read (spinlock_aprog cid) pc
+      (BExp_Den $ BVar "crit" $ BType_Imm Bit64)
+Proof
+  rpt gen_tac >> strip_tac
+  >> EVAL_TAC
+  >> fs[]
+QED
+
+(* all possible steps of the abstract spinlock
+ * sl_step (block,pc) (block',pc') *)
+(* TODO rename control flow *)
+(* TODO automate *)
+
+Inductive asl_step:
+     asl_step (BL_Address $ Imm64 0w,0n) (BL_Address $ Imm64 0w,1n)
+  /\ asl_step (BL_Address $ Imm64 0w,1)  (BL_Address $ Imm64 0w,2)
+  /\ asl_step (BL_Address $ Imm64 0w,2)  (BL_Address $ Imm64 0w,0)
+  /\ asl_step (BL_Address $ Imm64 0w,2)  (BL_Address $ Imm64 4w,0)
+  /\ asl_step (BL_Address $ Imm64 4w,0)  (BL_Address $ Imm64 8w,0)
+End
+
+(* pc is reachable for bir_spinlock from its first pc *)
+(* TODO automate *)
+
+Definition reachable_asl_def:
+  reachable_asl pc =
+    !bpt. bpt = bst_pc_tuple pc ==>
+    bpt = (BL_Address $ Imm64 0w,0) \/ bpt = (BL_Address $ Imm64 0w,1) \/
+    bpt = (BL_Address $ Imm64 0w,2) \/ bpt = (BL_Address $ Imm64 4w,0) \/
+    bpt = (BL_Address $ Imm64 8w,0)
+End
+
+
+(* pc within crit region *)
+(* the abstract program contains only one statement, thus behaves atomically *)
+Definition in_crit_asl_def:
+  in_crit_asl pc <=> reachable_asl pc
+End
+
+(* pc within lock region *)
+Definition in_lock_asl_def:
+  in_lock_asl pc <=>
+    reachable_asl pc
+    /\ !n. bst_pc_tuple pc = (BL_Address $ Imm64 0w,n) ==> 0 < n
+End
+
+(* pc not in lock or unlock region *)
+Definition outside_un_lock_asl_def:
+  outside_un_lock_asl pc <=>
+    !x n. bst_pc_tuple pc = (BL_Address $ Imm64 x,n)
+    ==>  (x,n) = (0w,0)
+      \/ (x,n) = (4w,0)
+      \/ (x,n) = (8w,0)
+End
+
+val _ = export_theory();
